hooray seq_cps works now.  ok so this is just a special case of omnisemantics

bedrock2/src/bedrock2/Semantics.v
@@ -136,25 +136,25 @@ Module exec. Section WithParams.
 
   Definition nst := list (word * mem). (*'nondeterministic state', list of stackalloc addrs*)
 
-  Implicit Types post : (nst -> trace) -> (nst -> mem) -> (nst -> locals) -> Prop. (* COQBUG: unification finds Type instead of Prop and fails to downgrade *)
+  Implicit Types post : (nst -> Prop) -> (nst -> trace) -> (nst -> mem) -> (nst -> locals) -> Prop. (* COQBUG: unification finds Type instead of Prop and fails to downgrade *)
   Inductive exec: cmd -> (nst -> Prop) -> (nst -> trace) -> (nst -> mem) -> (nst -> locals) ->
-                  ((nst -> trace) -> (nst -> mem) -> (nst -> locals) -> Prop) -> Prop :=
+                  ((nst -> Prop) -> (nst -> trace) -> (nst -> mem) -> (nst -> locals) -> Prop) -> Prop :=
   | skip: forall H t m l post,
-      post t m l ->
+      post H t m l ->
       exec cmd.skip H t m l post
   | set: forall x e H t m l post v,
       (forall n, H n -> eval_expr (m n) (l n) e = Some (v n)) ->
-      post t m (fun n => map.put (l n) x (v n)) ->
+      post H t m (fun n => map.put (l n) x (v n)) ->
       exec (cmd.set x e) H t m l post
   | unset: forall x H t m l post,
-      post t m (fun n => map.remove (l n) x) ->
+      post H t m (fun n => map.remove (l n) x) ->
       exec (cmd.unset x) H t m l post
   | store: forall sz ea ev H t m l post a v m',
       (forall n, H n ->
             eval_expr (m n) (l n) ea = Some (a n) /\
               eval_expr (m n) (l n) ev = Some (v n) /\
               store sz (m n) (a n) (v n) = Some (m' n)) ->
-      post t m' l ->
+      post H t m' l ->
       exec (cmd.store sz ea ev) H t m l post
   | stackalloc: forall x nbytes body H t mSmall l post,
       Z.modulo nbytes (bytes_per_word width) = 0 ->
@@ -177,13 +177,13 @@ Module exec. Section WithParams.
              | (a, mStack) :: n' => map.put (l n') x a
              | _ => map.empty
              end)
-          (fun t' mCombined' l' =>
+          (fun H' t' mCombined' l' =>
              forall a mStack,
                exists mSmall' mStack',
-                 (forall n, H n ->
+                 (forall n, H' n ->
                        anybytes a nbytes (mStack' n) /\
                          map.split (mCombined' ((a, mStack) :: n)) (mSmall' n) (mStack' n)) /\
-                   post (fun n => t' ((a, mStack) :: n)) mSmall' (fun n => l' ((a, mStack) :: n))) ->
+                   post (fun n => H' ((a, mStack) :: n)) (fun n => t' ((a, mStack) :: n)) mSmall' (fun n => l' ((a, mStack) :: n))) ->
       exec (cmd.stackalloc x nbytes body) H t mSmall l post
   | if_true_false: forall H t m l e c1 c2 post v,
       (forall n, H n ->
@@ -193,14 +193,14 @@ Module exec. Section WithParams.
       exec (cmd.cond e c1 c2) H t m l post
   | seq: forall c1 c2 H t m l post mid,
       exec c1 H t m l mid ->
-      (forall t' m' l', mid t' m' l' -> exec c2 H t' m' l' post) ->
+      (forall H' t' m' l', mid H' t' m' l' -> exec c2 H' t' m' l' post) ->
       exec (cmd.seq c1 c2) H t m l post
   | while_true_false: forall e c H t m l post mid v,
       (forall n, H n ->
             eval_expr (m n) (l n) e = Some (v n)) ->
-      (forall n, word.unsigned (v n) = 0 /\ H n -> post n (t n) (m n) (l n)) ->
+      post (fun n => word.unsigned (v n) = 0 /\ H n) t m l ->
       exec c (fun n => word.unsigned (v n) <> 0 /\ H n) t m l mid ->
-      (forall t' m' l', exec (cmd.while e c) (fun n => mid n (t' n) (m' n) (l' n)) t' m' l' post) ->
+      (forall H' t' m' l', mid H' t' m' l' -> exec (cmd.while e c) H' t' m' l' post) ->
       exec (cmd.while e c) H t m l post
   (* | call: forall binds fname arges t m l post params rets fbody args lf mid, *)
   (*     map.get e fname = Some (params, rets, fbody) -> *)
@@ -225,8 +225,8 @@ Module exec. Section WithParams.
   Context {word_ok: word.ok word} {mem_ok: map.ok mem} {ext_spec_ok: ext_spec.ok ext_spec}.
 
   Lemma seq_cps: forall c1 c2 H t m l post,
-      exec c1 H t m l (fun n t' m' l' => exec c2 t' m' l' post) ->
-      exec (cmd.seq c1 c2) t m l post.
+      exec c1 H t m l (fun H' t' m' l' => exec c2 H' t' m' l' post) ->
+      exec (cmd.seq c1 c2) H t m l post.
   Proof. intros. eauto using seq. Qed.
 
   Lemma weaken: forall t l m s post1,
